Ntree.v
@@ -1,0 +1,775 @@
+Require Import Etacs.
+Require Import FunctionalExtensionality.
+Require Import Picinae_theory.
+Require Import Arith.
+Require Import NArith.
+Require Import List.
+Require Import Bool.
+
+Open Scope N.
+
+(* Some functions stuff *)
+Definition ident {A} (a: A): A := a.
+Definition compose {A} {B} {C} (fn1: B -> C) (fn2: A -> B) (a: A): C := fn1 (fn2 a).
+Definition injective {A} {B} (fn: A -> B) :=
+  forall p1 p2 (EQ: fn p1 = fn p2), p1 = p2.
+
+Ltac prove_injective :=
+  match goal with
+  | [|- injective _] =>
+      let p1 := fresh "p1" in
+      let p2 := fresh "p2" in
+      let EQ := fresh "EQ" in
+      intros p1 p2 EQ; repeat first
+        [ match type of EQ with
+          | ?fn _ = _ =>
+              match goal with
+              | INJ: injective fn |- _ => apply INJ in EQ
+              | _ => injection EQ; clear EQ; intros EQ
+              end
+          end
+        | trivial2
+        ]
+  end.
+
+
+Theorem compose_ident_l: forall A B (fn: A -> B), compose ident fn = fn.
+Proof.
+  intros. erewrite functional_extensionality. reflexivity.
+  intros. unfold compose, ident. reflexivity.
+Qed.
+
+Theorem compose_ident_r: forall A B (fn: A -> B), compose fn ident = fn.
+Proof.
+  intros. erewrite functional_extensionality. reflexivity.
+  intros. unfold compose, ident. reflexivity.
+Qed.
+
+Theorem injective_contra: forall A B (fn: A -> B) p1 p2 (INJ: injective fn)
+  (NEQ: p1 <> p2), fn p1 <> fn p2.
+Proof.
+  intros. revert NEQ. contrapositive INJ.
+Qed.
+
+(* Some lists stuff and related theorems *)
+Definition is_empty {A} (l: list A) :=
+  match l with
+  | nil => true
+  | _ => false
+  end.
+
+Theorem NoDup_app: forall A (l l': list A) (ND1: NoDup l) (ND2: NoDup l')
+  (CrossNE: forall a b (InL: In a l) (InL': In b l'), a <> b),
+  NoDup (l ++ l').
+Proof.
+  induction l; intros.
+  - assumption.
+  - inversion ND1. subst. clear ND1. constructor; fold (app l).
+
+    (* a cannot be in l or l' *)
+    intros Contra. apply in_app_or in Contra. destruct Contra. tauto.
+    einstantiate CrossNE. constructor. reflexivity. eassumption. invalid H0.
+
+    (* IH *)
+    apply IHl; try eassumption. intros. apply CrossNE; try right; assumption.
+Qed.
+
+Theorem in_map_inj_iff: forall A B (f: A -> B) l x (INJ: injective f),
+  In (f x) (map f l) <-> In x l.
+Proof.
+  intros. split; [|apply in_map]. intros InMl. apply in_map_iff in InMl.
+  destruct InMl as [x' [EQ In]]. apply INJ in EQ. subst. assumption.
+Qed.
+
+Lemma NoDup_map_inj: forall (A B : Type) (f : A -> B) (l : list A)
+  (INJ: injective f) (ND: NoDup l), NoDup (map f l).
+Proof.
+  induction l; intros.
+  - constructor.
+  - simpl. inversion ND. subst. constructor.
+
+    (* f a is not in map *)
+    intro Contra. apply in_map_inj_iff in Contra. contradiction H1.
+    prove_injective.
+
+    (* NoDup of map *)
+    apply IHl; assumption.
+Qed.
+
+Theorem map_inj: forall (A B : Type) (f : A -> B)
+  (INJ: injective f), injective (map f).
+Proof.
+  intros. prove_injective. revert p2 EQ. induction p1; intros.
+  - destruct p2; [|discriminate]. reflexivity.
+  - destruct p2. discriminate. simpl in EQ. inversion EQ. apply INJ in H0.
+    subst. f_equal. apply IHp1. assumption.
+Qed.
+
+Definition list_equiv {A} (l1 l2: list A) := incl l1 l2 /\ incl l2 l1.
+Theorem list_nequiv_1: forall A (h: A) t, list_equiv nil (h::t) -> False.
+Proof. intros. destruct H. einversion (H0 h). left. reflexivity. Qed.
+
+Theorem list_nequiv_2: forall A (h: A) t, list_equiv (h::t) nil -> False.
+Proof. intros. destruct H. einversion (H h). left. reflexivity. Qed.
+
+Theorem list_equiv_refl: forall A (l: list A), list_equiv l l.
+Proof. intros. split; apply incl_refl. Qed.
+
+Theorem list_equiv_symm: forall A (l1 l2: list A),
+  list_equiv l1 l2 <-> list_equiv l2 l1.
+Proof. intros. split; intros [? ?]; split; assumption. Qed.
+
+Theorem list_equiv_tran: forall A (l1 l2 l3: list A),
+  list_equiv l1 l2 -> list_equiv l2 l3 -> list_equiv l1 l3.
+Proof.
+  intros A l1 l2 l3 [Incl12 Incl21] [Incl23 Incl32].
+  split; eapply incl_tran; eassumption.
+Qed.
+
+Theorem incl_cons_2: forall {A} {a : A} {l m : list A},
+  In a l -> incl l m -> incl (a :: l) m.
+Proof. intros. intros a0 InA. inversion InA; subst; apply H0; assumption. Qed.
+
+Theorem incl_map_iff: forall {A B} (f: A -> B) {l1 l2: list A}
+  (INJ: injective f), incl l1 l2 <-> incl (map f l1) (map f l2).
+Proof.
+  split. apply incl_map. intros Incl a In1. specialize (Incl (f a)).
+  eapply in_map_inj_iff, Incl, in_map_inj_iff; assumption.
+Qed.
+
+Theorem list_equiv_map_iff: forall {A B} (f: A -> B) {l1 l2: list A}
+  (INJ: injective f), list_equiv l1 l2 <-> list_equiv (map f l1) (map f l2).
+Proof.
+  split; intros EQV; destruct EQV as [EQV1 EQV2];
+  split; (erewrite <- incl_map_iff + erewrite incl_map_iff); eassumption.
+Qed.
+
+Theorem list_equiv_cons: forall {A} {l1 l2} (a: A) (In1: In a l1),
+  list_equiv l1 l2 <-> list_equiv (a::l1) l2.
+Proof.
+  split; intros EQV.
+  - destruct EQV as [Incl12 Incl21]. split; [apply incl_cons_2|apply incl_tl];
+    assumption.
+  - destruct EQV as [Incl12 Incl21]. split.
+    + intros a' In1'. apply Incl12. right. assumption.
+    + intros a' In2'. einstantiate trivial (Incl21 a') as In1'.
+      inversion In1'; subst; assumption.
+Qed.
+
+Theorem list_equiv_remove: forall {A} (a: A) {e: EqDec A} l1 l2
+  (EQV: list_equiv l1 l2), list_equiv (remove iseq a l1) (remove iseq a l2).
+Proof. intros. destruct EQV. split; apply remove_incl; assumption. Qed.
+
+Theorem list_equiv_remove_inv: forall {A} (a: A) {e: EqDec A} l1 l2
+  (In1: In a l1) (In2: In a l2)
+  (EQV: list_equiv (remove iseq a l1) (remove iseq a l2)), list_equiv l1 l2.
+Proof.
+  intros. destruct EQV. split; intros a' In'; destruct (a' == a); subst; trivial2;
+  ((einstantiate (H a') + einstantiate (H0 a'));
+  [apply in_in_remove|eapply in_remove]; eassumption).
+Qed.
+
+Theorem list_equiv_partition: forall A {e: EqDec A} (l1_1 l1_2 l2_1 l2_2: list A)
+  (EQV: list_equiv (l1_1 ++ l1_2) (l2_1 ++ l2_2))
+  (DISJ1: forall a b (In1: In a l1_1) (In2: In b l2_2), a <> b)
+  (DISJ2: forall a b (In1: In a l2_1) (In2: In b l1_2), a <> b),
+  list_equiv l1_1 l2_1 /\ list_equiv l1_2 l2_2.
+Proof.
+  induction l1_1; intros.
+  - destruct l2_1. split; [apply list_equiv_refl|trivial2].
+    simpl in *. destruct EQV as [_ Contra].
+    destruct (DISJ2 a a). left. reflexivity. apply Contra. left. reflexivity.
+    reflexivity.
+  - destruct (in_dec iseq a l1_1).
+    + (* a is still in l1_1 *) simpl in EQV. rewrite <- list_equiv_cons in EQV;
+      [|apply in_or_app; left; assumption]. einstantiate trivial IHl1_1.
+      intros. apply DISJ1; [right|]; assumption.
+      rewrite <- list_equiv_cons; assumption.
+    + (* a no longer is in l1_1. a must only be in l2_1 *)
+      assert (N2_2: ~ In a l2_2).
+        intro In22. edestruct (DISJ1 a a); trivial2. left. reflexivity.
+      assert (In21: In a l2_1). destruct EQV. einstantiate (H a) as In.
+        left. reflexivity. apply in_app_or in In. destruct In. assumption.
+        contradiction N2_2.
+      assert (N1_2: ~ In a l1_2). intro In12. edestruct (DISJ2 a a); trivial2.
+
+      apply (list_equiv_remove a) in EQV as EQV2.
+      simpl in EQV2. vreflexivity a. repeat rewrite remove_app in EQV2.
+      rewrite notin_remove in EQV2 by assumption.
+      einstantiate trivial IHl1_1 as IHl1_1.
+      (* DISJ1' *)
+      intros. apply DISJ1. right. assumption. eapply in_remove; eassumption.
+      (* DISJ2' *)
+      intros. apply DISJ2; eapply in_remove; eassumption.
+
+      (* From a remove operation, we show they are equivalent *)
+      destruct IHl1_1 as [EQV_1 EQV_2].
+      repeat rewrite notin_remove in EQV_2 by assumption. split; [|assumption].
+      eapply list_equiv_remove_inv; try left; trivial2.
+      simpl. vreflexivity a. rewrite notin_remove; assumption.
+Qed.
+
+Theorem list_app_partition: forall A (l1_1 l1_2 l2_1 l2_2: list A)
+  (EQ: (l1_1 ++ l1_2) = (l2_1 ++ l2_2))
+  (DISJ1: forall a b (In1: In a l1_1) (In2: In b l2_2), a <> b)
+  (DISJ2: forall a b (In1: In a l2_1) (In2: In b l1_2), a <> b),
+  l1_1 = l2_1 /\ l1_2 = l2_2.
+Proof.
+  induction l1_1; intros.
+  - destruct l2_1. split; trivial2. simpl in *. subst.
+    destruct (DISJ2 a a); try left; reflexivity.
+  - destruct l2_1. simpl in *. subst. destruct (DISJ1 a a); try left; reflexivity.
+    simpl in EQ. inversion EQ. subst. einstantiate trivial IHl1_1 as IHl1_1.
+    (* DISJ1' *) intros. apply DISJ1; try right; assumption.
+    (* DISJ2' *) intros. apply DISJ2; try right; assumption.
+    destruct IHl1_1 as [EQ1 EQ2]. subst. split; reflexivity.
+Qed.
+
+
+Inductive treeP_ (V: Type) :=
+  | TPleaf (val: V)
+  | TP0 (t0: treeP_ V) (val: option V)
+  | TP1 (t1: treeP_ V) (val: option V)
+  | TP01 (t0 t1: treeP_ V) (val: option V).
+
+Definition treeP V := option (treeP_ V).
+Definition treeP_nil {V}: treeP V := None.
+
+Arguments TPleaf {_} _.
+Arguments TP0 {_} _ _.
+Arguments TP1 {_} _ _.
+Arguments TP01 {_} _ _ _.
+
+Inductive treeN (V: Type) :=
+  | TN (v0: option V) (tp: treeP V).
+Arguments TN {_} _ _.
+
+Definition treeN_nil {V}: treeN V := TN None treeP_nil.
+
+Instance positive_EqDec: EqDec positive :=
+  { iseq := Pos.eq_dec }.
+
+Program Instance option_EqDec A `(e: EqDec A): EqDec (option A).
+Next Obligation. decide equality. apply iseq. Defined.
+
+Program Instance treeP__EqDec V `(e: EqDec V): EqDec (treeP_ V).
+Next Obligation. decide equality; apply iseq. Defined.
+
+Program Instance treeP_EqDec V `(e: EqDec V): EqDec (treeP V).
+Next Obligation. decide equality; apply iseq. Defined.
+
+Program Instance treeN_EqDec V `(e: EqDec V): EqDec (treeN V).
+Next Obligation. decide equality; apply iseq. Defined.
+
+Definition tempty_p {V} (t: treeP V) :=
+  match t with
+  | Some _ => false
+  | None => true
+  end.
+
+Definition tempty_n {V} (t: treeN V) :=
+  match t with
+  | TN (Some _) _ => false
+  | TN None tp => tempty_p tp
+  end.
+
+Definition textract_node_p {V} (t: treeP V): (treeP V * treeP V * option V) :=
+  match t with
+  | Some t =>
+      match t with
+      | TPleaf v =>  (None, None, Some v)
+      | TP0 t0 ov => (Some t0, None, ov)
+      | TP1 t1 ov => (None, Some t1, ov)
+      | TP01 t0 t1 ov => (Some t0, Some t1, ov)
+      end
+  | None => (None, None, None)
+  end.
+
+Definition tupdate_node_p {V} (t0: treeP V) (t1: treeP V) (ov: option V): treeP V :=
+  match t0, t1 with
+  | None, None =>
+      match ov with
+      | None => None
+      | Some v => Some (TPleaf v)
+      end
+  | Some t0, None => Some (TP0 t0 ov)
+  | None, Some t1 => Some (TP1 t1 ov)
+  | Some t0, Some t1 => Some (TP01 t0 t1 ov)
+  end.
+
+Fixpoint tget_p {V} (t: treeP V) (key: positive) {struct key}: option V :=
+  let '(t0, t1, ov) := textract_node_p t in
+  match key with
+  | xO key' => tget_p t0 key'
+  | xI key' => tget_p t1 key'
+  | xH => ov
+  end.
+
+Definition tget_n {V} (t: treeN V) (key: N): option V :=
+  match t with
+  | TN ov tp =>
+      match key with
+      | N0 => ov
+      | Npos key' => tget_p tp key'
+      end
+  end.
+
+Definition tcontains_p {V} (t: treeP V) (key: positive): bool :=
+  match tget_p t key with
+  | Some _ => true
+  | None => false
+  end.
+
+Definition tcontains_n {V} (t: treeN V) (key: N): bool :=
+  match tget_n t key with
+  | Some _ => true
+  | None => false
+  end.
+
+Fixpoint tupdate_p {V} (t: treeP V) (key: positive) (val: V): treeP V :=
+  let '(t0, t1, ov) := textract_node_p t in
+  match key with
+  | xO key' => tupdate_node_p (tupdate_p t0 key' val) t1 ov
+  | xI key' => tupdate_node_p t0 (tupdate_p t1 key' val) ov
+  | xH => tupdate_node_p t0 t1 (Some val)
+  end.
+
+Definition tupdate_n {V} (t: treeN V) (key: N) (val: V): treeN V :=
+  match t with
+  | TN ov tp =>
+      match key with
+      | N0 => TN (Some val) tp
+      | Npos key' => TN ov (tupdate_p tp key' val)
+      end
+  end.
+
+Notation "t [Ⓝ  x := y ]" := (tupdate_n t x y) (at level 50, left associativity).
+Notation "t [Ⓟ  x := y ]" := (tupdate_p t x y) (at level 50, left associativity).
+Notation "t Ⓝ[ x ]" := (tget_n t x) (at level 10).
+Notation "t Ⓟ[ x ]" := (tget_p t x) (at level 10).
+
+Fixpoint tkeys_p_ {V} (t: treeP_ V) (fn: positive -> positive): list positive :=
+  let fn0 := compose fn xO in
+  let fn1 := compose fn xI in
+  match t with
+  | TPleaf v => (fn xH) :: nil
+  | TP0 t0 ov =>
+      match ov with
+      | Some v => fn xH :: nil
+      | None => nil
+      end ++ tkeys_p_ t0 fn0
+  | TP1 t1 ov =>
+      match ov with
+      | Some v => fn xH :: nil
+      | None => nil
+      end ++ tkeys_p_ t1 fn1
+  | TP01 t0 t1 ov =>
+      match ov with
+      | Some v => fn xH :: nil
+      | None => nil
+      end ++ tkeys_p_ t0 fn0 ++ tkeys_p_ t1 fn1
+  end.
+
+Definition tkeys_p {V} (t: treeP V) (fn: positive -> positive): list positive :=
+  match t with
+  | Some t => tkeys_p_ t fn
+  | None => nil
+  end.
+
+Definition tkeys_n {V} (t: treeN V): list N :=
+  match t with
+  | TN v0 tp =>
+      match v0 with
+      | None => nil
+      | Some v => 0 :: nil
+      end ++ map Npos (tkeys_p tp ident)
+  end.
+
+Theorem textract_update_node_p_inv: forall V t0 t1 (ov: option V),
+  (textract_node_p (tupdate_node_p t0 t1 ov)) = (t0, t1, ov).
+Proof. intros. destruct t0, t1, ov; reflexivity. Qed.
+
+Theorem tupdate_extract_node_p_inv: forall V t t0 t1 (ov: option V)
+  (EXT: textract_node_p t = (t0, t1, ov)),
+  (tupdate_node_p t0 t1 ov) = t.
+Proof. intros. destruct t as [[| | |]|]; inversion EXT; subst; reflexivity. Qed.
+
+Theorem tupdate_p_updated: forall V k t (v: V),
+  tget_p (tupdate_p t k v) k = Some v.
+Proof.
+  induction k; intros; simpl; destruct (textract_node_p t) as [[t0 t1] ov];
+  rewrite textract_update_node_p_inv; solve [apply IHk | reflexivity].
+Qed.
+
+Theorem tupdate_n_updated: forall V k t (v: V),
+  tget_n (tupdate_n t k v) k = Some v.
+Proof.
+  intros. destruct t as [v0 tp]. unfold tget_n, tupdate_n.
+  destruct k; try solve [reflexivity|apply tupdate_p_updated].
+Qed.
+
+Theorem tupdate_p_frame: forall V k k0 t (v: V) (NEQ: k0 <> k),
+  tget_p (tupdate_p t k v) k0 = tget_p t k0.
+Proof.
+  induction k; intros; simpl; destruct textract_node_p as [[t0 t1] ov] eqn: EXT;
+  (* if k0 != k by structure, very trivial *)
+  destruct k0; simpl; rewrite textract_update_node_p_inv, EXT; trivial2.
+  - (* ~1 *) apply IHk. intro Contra. subst. invalid NEQ.
+  - (* ~0 *) apply IHk. intro Contra. subst. invalid NEQ.
+  - (* H *) invalid NEQ.
+Qed.
+
+Theorem tupdate_n_frame: forall V k k0 t (v: V) (NEQ: k0 <> k),
+  tget_n (tupdate_n t k v) k0 = tget_n t k0.
+Proof.
+  intros. destruct t. simpl.
+  destruct k, k0; try solve [invalid NEQ | reflexivity].
+  apply tupdate_p_frame. intro Contra. subst. invalid NEQ.
+Qed.
+
+Theorem tkeys_p_tkeys_extract: forall V (t t0 t1: treeP V) ov fn
+  (EXT: textract_node_p t = (t0, t1, ov)),
+  tkeys_p t fn = match ov with Some v => (fn xH :: nil) | None => nil end ++
+    tkeys_p t0 (compose fn xO) ++ tkeys_p t1 (compose fn xI).
+Proof.
+  intros. destruct t as [[| | |]|]; inversion EXT; subst;
+      repeat rewrite app_nil_r; reflexivity.
+Qed.
+
+Lemma tkeys_p_tupdate_node: forall V t0 t1 (ov: option V) fn,
+  tkeys_p (tupdate_node_p t0 t1 ov) fn =
+  match ov with
+  | Some _ => fn 1%positive :: nil
+  | None => nil
+  end ++ tkeys_p t0 (compose fn xO) ++ tkeys_p t1 (compose fn xI).
+Proof.
+  intros. remember (tupdate_node_p _ _ _) as t. apply tkeys_p_tkeys_extract.
+  subst. rewrite textract_update_node_p_inv. reflexivity.
+Qed.
+
+Theorem treeP_ind2: forall {V} (t: treeP V) (P: treeP V -> Prop)
+  (BASE: P None) (IND: forall (t' tx0 tx1: treeP V) ov
+    (IHt0: P tx0) (IHt1: P tx1) (EXT: textract_node_p t' = (tx0, tx1, ov)), P t'),
+  P t.
+Proof.
+  destruct t as [t|]; [|intros; assumption]. induction t; intros.
+  - (* leaf *) eapply IND; trivial2.
+  - (* TP0 *) eapply IND; [|eassumption|reflexivity]. apply IHt; eassumption.
+  - (* TP1 *) eapply IND; [eassumption| |reflexivity]. apply IHt; eassumption.
+  - (* TP01 *) eapply IND; [| |reflexivity]. apply IHt1; eassumption.
+    apply IHt2; eassumption.
+Qed.
+
+Theorem tkeys_p_fn_res: forall V (t: treeP V) p fn
+  (InKeys: In p (tkeys_p t fn)), exists p0, p = fn p0.
+Proof.
+  intro. induction t as [|t tx0 tx1] using treeP_ind2; intros.
+  - inversion InKeys.
+  - erewrite tkeys_p_tkeys_extract in InKeys by eassumption.
+    repeat rewrite in_app_iff in InKeys. destruct InKeys as [InOV|[InX0|InX1]].
+    + destruct ov; inversion InOV; subst; try inversion H. eexists. reflexivity.
+    + einversion trivial IHt1. eexists. reflexivity.
+    + einversion trivial IHt2. eexists. reflexivity.
+Qed.
+
+Theorem tkeys_p_map: forall V (t: treeP V) fn,
+  tkeys_p t fn = map fn (tkeys_p t ident).
+Proof.
+  intros until t. induction t as [|t tx0 tx1] using treeP_ind2; intros.
+  - reflexivity.
+  - repeat erewrite (tkeys_p_tkeys_extract _ t) by eassumption.
+    repeat rewrite map_app. rewrite IHt1, IHt2. symmetry.
+    rewrite IHt1, IHt2. repeat rewrite map_map. f_equal. destruct ov; reflexivity.
+Qed.
+
+Lemma tkeys_nexists_neq_h: forall V (val: option V) fn (p: positive)
+    (INJ: injective fn) (NEQ: p <> 1%positive),
+    (existsb (Pos.eqb (fn p))
+        match val with
+        | Some _ => fn 1 :: nil
+        | None => nil
+        end = false)%positive.
+Proof.
+  intros. destruct val; try reflexivity. simpl. rewrite orb_false_r.
+  apply Pos.eqb_neq. apply injective_contra; trivial2.
+Qed.
+
+Lemma tkeys_nexists_neq_0: forall V fn (p: positive) (t: treeP V)
+    (INJ: injective fn) (NEQ: forall p0, (p0~0)%positive <> p),
+    (existsb (Pos.eqb (fn p))
+      (tkeys_p t (fun p0 : positive => fn (p0~0)%positive)) = false)%positive.
+Proof.
+  intros. apply not_true_is_false. intro Contra.
+  apply existsb_exists, Exists_exists in Contra. revert Contra.
+  apply Forall_Exists_neg, Forall_forall. intros p0 InKeys Contra.
+  einversion trivial tkeys_p_fn_res as [p']. apply Pos.eqb_eq in Contra.
+  apply INJ in Contra. subst. specialize (NEQ p'). invalid NEQ.
+Qed.
+
+Lemma tkeys_nexists_neq_1: forall V fn (p: positive) (t: treeP V)
+    (INJ: injective fn) (NEQ: forall p0, (p0~1)%positive <> p),
+    (existsb (Pos.eqb (fn p))
+      (tkeys_p t (fun p0 : positive => fn (p0~1)%positive)) = false)%positive.
+Proof.
+  intros. apply not_true_is_false. intro Contra.
+  apply existsb_exists, Exists_exists in Contra. revert Contra.
+  apply Forall_Exists_neg, Forall_forall. intros p0 InKeys Contra.
+  einversion trivial tkeys_p_fn_res as [p']. apply Pos.eqb_eq in Contra.
+  apply INJ in Contra. subst. specialize (NEQ p'). invalid NEQ.
+Qed.
+
+Theorem tkeys_p_get: forall V p fn (t: treeP V)
+  (INJ: injective fn),
+  existsb (Pos.eqb (fn p)) (tkeys_p t fn) = tcontains_p t p.
+Proof.
+  unfold tcontains_p. induction p; intros; simpl;
+  destruct textract_node_p as [[t0 t1] ov] eqn: EXT;
+  erewrite tkeys_p_tkeys_extract by eassumption.
+  - (* ~1 *) rewrite existsb_app, existsb_app, tkeys_nexists_neq_h,
+    tkeys_nexists_neq_0 by trivial2. simpl.
+    apply (IHp (fun p => fn (xI p))). prove_injective.
+  - (* ~0 *) rewrite existsb_app, existsb_app, tkeys_nexists_neq_h,
+      tkeys_nexists_neq_1 by trivial2. simpl.
+    rewrite orb_false_r. apply (IHp (fun p => fn (xO p))). prove_injective.
+  - (* H *) rewrite existsb_app, existsb_app, tkeys_nexists_neq_0,
+      tkeys_nexists_neq_1 by trivial2. simpl.
+    rewrite orb_false_r. destruct ov; simpl. rewrite Pos.eqb_refl.
+    reflexivity. reflexivity.
+Qed.
+
+Theorem tkeys_n_get: forall V n (t: treeN V),
+  existsb (N.eqb n) (tkeys_n t) = tcontains_n t n.
+Proof.
+  unfold tcontains_n, tget_n. intros. destruct t, n; simpl.
+  - (* 0 *) rewrite existsb_app.
+    eassert (EXB2: existsb _ (map _ _) = false); [|rewrite EXB2].
+      apply not_true_is_false. intro Contra.
+      apply existsb_exists, Exists_exists in Contra. revert Contra.
+      apply Forall_Exists_neg, Forall_forall. intros n0 InKeys Contra.
+      apply N.eqb_eq in Contra. subst. apply in_map_iff in InKeys.
+      destruct InKeys as [x [Contra _]]. discriminate.
+    rewrite orb_false_r. destruct v0; reflexivity.
+  - (* Pos *) rewrite existsb_app. eassert (EXB1: existsb _ _ = false);
+      [|rewrite EXB1]. destruct v0; reflexivity.
+    simpl. fold (tcontains_p tp p). assert (injective (@ident positive)).
+    prove_injective.
+    destruct tcontains_p eqn: TC;
+      erewrite <- tkeys_p_get with (fn := ident) in TC by assumption.
+    + (* true *) apply existsb_exists in TC. apply existsb_exists. unfold ident in *.
+      destruct TC as [p' [InKeys Eq]]. apply Pos.eqb_eq in Eq. subst. eexists.
+      rewrite N.eqb_eq. split; [|reflexivity]. apply in_map_iff.
+      eexists. split. reflexivity. assumption.
+    + (* false *) apply not_true_is_false. apply not_true_iff_false in TC.
+      intro Contra. apply TC. clear TC. apply existsb_exists in Contra.
+      apply existsb_exists. unfold ident in *. destruct Contra as [p' [InKeys Eq]].
+      apply N.eqb_eq in Eq. subst. eexists. rewrite Pos.eqb_eq.
+      split; [|reflexivity]. apply in_map_iff in InKeys.
+      destruct InKeys as [p' [EQ In]]. inversion EQ. subst. assumption.
+Qed.
+
+Theorem tkeys_p_nodup: forall V (t: treeP V) fn (INJ: injective fn),
+  NoDup (tkeys_p t fn).
+Proof.
+  intros until t. induction t as [|t tx0 tx1] using treeP_ind2; intros.
+  - constructor.
+  - repeat erewrite (tkeys_p_tkeys_extract _ t) by eassumption.
+    rewrite tkeys_p_map, (tkeys_p_map _ tx1). unfold compose.
+    (* Prove no duplicates when we merge t1 and t2 *)
+    eassert (NoDup _); [|destruct ov; simpl; [constructor|]; try eassumption].
+    apply NoDup_app. apply NoDup_map_inj. prove_injective. apply IHt1. prove_injective.
+    apply NoDup_map_inj. prove_injective. apply IHt2. prove_injective. intros.
+    apply in_map_iff in InL, InL'. destruct InL as [a' [EQa INt1]].
+    destruct InL' as [b' [EQb INt2]]. subst. intros Contra. apply INJ in Contra.
+    inversion Contra.
+
+    (* Prove 1 is not in the merged t1/t2 *)
+    intros Contra. apply in_app_or in Contra. destruct Contra as [C|C];
+    apply in_map_iff in C; destruct C as [a [EQa INt]];
+    apply INJ in EQa; inversion EQa.
+Qed.
+
+Theorem tkeys_n_nodup: forall V (t: treeN V), NoDup (tkeys_n t).
+Proof.
+  intros. unfold tkeys_n. destruct t.
+  assert (NoDup (map N.pos (tkeys_p tp ident))).
+    apply NoDup_map_inj; try apply tkeys_p_nodup; prove_injective.
+  destruct v0; [|assumption]. constructor; [|assumption]. intros Contra.
+  apply in_map_iff in Contra. destruct Contra as [a [EQa INt2]]. discriminate.
+Qed.
+
+Theorem tupdate_p_idempotent: forall V k (v: V) t (LU: tget_p t k = Some v),
+  (tupdate_p t k v) = t.
+Proof.
+  induction k; intros; simpl in *; destruct textract_node_p as [[tx0 tx1] ov] eqn: EXT.
+  - (* ~1 *) rewrite IHk; try apply tupdate_extract_node_p_inv; assumption.
+  - (* ~0 *) rewrite IHk; try apply tupdate_extract_node_p_inv; assumption.
+  - (* H *) subst. apply tupdate_extract_node_p_inv. assumption.
+Qed.
+
+Theorem tupdate_n_idempotent: forall V k (v: V) t (LU: tget_n t k = Some v),
+  (tupdate_n t k v) = t.
+Proof.
+  unfold tupdate_n. intros. destruct t, k; simpl in *.
+  - (* 0 *) subst. reflexivity.
+  - (* Pos *) rewrite tupdate_p_idempotent; trivial2.
+Qed.
+
+Lemma tree_p_disjoint_H_x01: forall V (val: option V) fn (t1 t2: treeP V) a b
+  (INJ: injective fn)
+  (In1: In a match val with
+             | Some _ => fn 1%positive :: nil
+             | None => nil
+             end)
+  (In2: In b
+    (tkeys_p t1 (fun p => fn (p~0)%positive) ++
+     tkeys_p t2 (fun p => fn (p~1)%positive))), a <> b.
+Proof.
+  intros. destruct val; inversion In1; inversion H. subst. clear H0.
+  apply in_app_or in In2. intro Contra. subst. rewrite tkeys_p_map,
+    (tkeys_p_map _ t2), in_map_iff, in_map_iff in In2.
+  destruct In2 as [[p [Contra _]]|[p [Contra _]]];
+  apply INJ in Contra; inversion Contra.
+Qed.
+
+Lemma tree_p_disjoint_x0_x1: forall V (val: option V) fn (t1 t2: treeP V) a b
+  (INJ: injective fn)
+  (In1: In a (tkeys_p t1 (fun p => fn (p~0)%positive)))
+  (In2: In b (tkeys_p t2 (fun p => fn (p~1)%positive))), a <> b.
+Proof.
+  intros. rewrite tkeys_p_map, in_map_iff in *.
+  destruct In1 as [a' [EQA _]]. destruct In2 as [b' [EQB _]]. subst.
+  apply injective_contra. assumption. discriminate.
+Qed.
+
+Theorem tkeys_p_equiv_equal: forall V (t1 t2: treeP V) fn (INJ: injective fn)
+  (EQV: list_equiv (tkeys_p t1 fn) (tkeys_p t2 fn)),
+    tkeys_p t1 fn = tkeys_p t2 fn.
+Proof.
+  intros until t1. induction t1 as [|t1 t1_x0 t1_x1 ov1] using treeP_ind2; intros.
+  - (* base *) simpl in EQV. destruct EQV as [_ Nil]. apply incl_l_nil in Nil.
+    rewrite Nil. reflexivity.
+  - (* induct *) destruct (textract_node_p t2) as [[t2_x0 t2_x1] ov2] eqn: EXT2.
+    repeat erewrite (tkeys_p_tkeys_extract _ t1) in * by eassumption.
+    repeat erewrite (tkeys_p_tkeys_extract _ t2) in * by eassumption.
+    apply (list_equiv_partition positive) in EQV;
+      try (intros; eapply tree_p_disjoint_H_x01; eassumption).
+    destruct EQV as [EQV_H EQV_x01].
+    apply (list_equiv_partition positive) in EQV_x01;
+      try (intros; eapply tree_p_disjoint_x0_x1; eassumption).
+    unfold compose in *. destruct EQV_x01 as [EQV_x0 EQV_x1]. f_equal; [|f_equal].
+    + destruct ov1, ov2; solve [ reflexivity
+      | destruct (list_nequiv_1 _ _ _ EQV_H)
+      | destruct (list_nequiv_2 _ _ _ EQV_H) ].
+    + apply IHt1_1. prove_injective. assumption.
+    + apply IHt1_2. prove_injective. assumption.
+Qed.
+
+Lemma tree_n_disjoint_0_pos: forall V (ov0: option V) (tp: treeP V) a b
+  (In1: In a match ov0 with
+       | Some _ => 0 :: nil
+       | None => nil
+       end)
+  (In2: In b (map N.pos (tkeys_p tp ident))), a <> b.
+Proof.
+  intros. destruct ov0; inversion In1; subst; try inversion H. intro EQ. subst.
+  apply in_map_iff in In2. destruct In2 as [n' [Contra _]]. discriminate.
+Qed.
+
+Theorem tkeys_n_equiv_equal: forall V (t1 t2: treeN V)
+  (EQV: list_equiv (tkeys_n t1) (tkeys_n t2)),
+    tkeys_n t1 = tkeys_n t2.
+Proof.
+  intros. destruct t1 as [t1_ov0 t1]. destruct t2 as [t2_ov0 t2].
+  simpl in *. apply (list_equiv_partition N) in EQV;
+    try (intros; eapply tree_n_disjoint_0_pos; eassumption).
+  destruct EQV as [EQV0 EQV_P]. f_equal.
+  - (* 0 *) destruct t1_ov0, t2_ov0; solve [ reflexivity
+    | destruct (list_nequiv_1 _ _ _ EQV0)
+    | destruct (list_nequiv_2 _ _ _ EQV0) ].
+  - (* Pos *) f_equal. apply tkeys_p_equiv_equal. prove_injective.
+    rewrite <- list_equiv_map_iff in EQV_P by prove_injective. assumption.
+Qed.
+
+Theorem is_empty_forallb: forall A (l: list A),
+  is_empty l = forallb (fun _ => false) l.
+Proof. intros. destruct l; reflexivity. Qed.
+
+Theorem tempty_p_keys_empty: forall V (t: treeP V) fn,
+  tempty_p t = is_empty (tkeys_p t fn).
+Proof.
+  intros. rewrite is_empty_forallb. revert_all. intros until t.
+  induction t as [|t t_x0 t_x1 ov] using treeP_ind2; intros.
+  - reflexivity.
+  - repeat erewrite (tkeys_p_tkeys_extract _ t) in * by eassumption.
+    repeat rewrite forallb_app. rewrite <- IHt1, <- IHt2.
+    destruct t as [[| | |]|]; inversion EXT; subst; try rewrite andb_false_r;
+    reflexivity.
+Qed.
+
+Lemma tupdate_p_nonempty: forall V (v: V) k t fn,
+  is_empty (tkeys_p (t [Ⓟ  k := v]) fn) = false.
+Proof.
+  intros. rewrite is_empty_forallb. revert_all. induction k; intros; simpl in *;
+  destruct (textract_node_p t) as [[tx0 tx1] ov] eqn: EXT;
+  repeat erewrite tkeys_p_tupdate_node; repeat rewrite forallb_app.
+  - (* ~1 *) rewrite IHk. repeat rewrite andb_false_r. reflexivity.
+  - (* ~0 *) rewrite IHk. repeat rewrite andb_false_r. reflexivity.
+  - (* H *) reflexivity.
+Qed.
+
+Theorem tkeys_p_inj: forall V (t1 t2: treeP V) fn
+  (VALS:forall v, tcontains_p t1 v = tcontains_p t2 v -> tget_p t1 v = tget_p t2 v)
+  (KEQ: tkeys_p t1 fn = tkeys_p t2 fn) (INJ: injective fn), t1 = t2.
+Proof.
+  intros until t1. induction t1 as [|t1 t1_x0 t1_x1 ov1] using treeP_ind2; intros.
+  - einstantiate (tempty_p_keys_empty V None) as Nil.
+    rewrite KEQ, <- tempty_p_keys_empty in Nil. destruct t2. discriminate.
+    reflexivity.
+  - erewrite (tkeys_p_tkeys_extract _ t1) in * by eassumption.
+    destruct (textract_node_p t2) as [[t2_x0 t2_x1] ov2] eqn: EXT2.
+    erewrite (tkeys_p_tkeys_extract _ t2) in * by eassumption.
+
+    (* Partition KEQ *)
+    apply list_app_partition in KEQ;
+      try (intros; eapply tree_p_disjoint_H_x01; eassumption).
+    destruct KEQ as [KEQ_H KEQ_x01].
+    apply list_app_partition in KEQ_x01;
+      try (intros; eapply tree_p_disjoint_x0_x1; eassumption).
+    destruct KEQ_x01 as [KEQ_x0 KEQ_x1].
+
+    (* ov1 = ov2 because of VALS and KEQ_H *)
+    assert (ov1 = ov2). destruct ov1, ov2; trivial2.
+      unfold tcontains_p in *. einstantiate (VALS xH) as VALS. simpl.
+      rewrite EXT, EXT2. reflexivity. simpl in VALS. rewrite EXT, EXT2 in VALS.
+      assumption. subst.
+
+    (* Now apply IH's *)
+    einstantiate trivial (IHt1_1 t2_x0). intros.
+      einstantiate (VALS (xO v)). unfold tcontains_p. simpl. rewrite EXT, EXT2.
+      assumption. simpl in H0. rewrite EXT, EXT2 in H0. assumption.
+      unfold compose. prove_injective.
+    einstantiate trivial (IHt1_2 t2_x1). intros.
+      einstantiate (VALS (xI v)). unfold tcontains_p. simpl. rewrite EXT, EXT2.
+      assumption. simpl in H1. rewrite EXT, EXT2 in H1. assumption.
+      unfold compose. prove_injective.
+
+    (* Parts are equal, so whole part is equal too *)
+    subst. erewrite <- (tupdate_extract_node_p_inv _ t1),
+      <- (tupdate_extract_node_p_inv _ t2) by eassumption. reflexivity.
+Qed.
+
+Theorem tkeys_n_inj: forall V (t1 t2: treeN V)
+  (VALS:forall v, tcontains_n t1 v = tcontains_n t2 v -> tget_n t1 v = tget_n t2 v)
+  (KEQ: tkeys_n t1 = tkeys_n t2), t1 = t2.
+Proof.
+  intros. destruct t1 as [t1_v0 t1]. destruct t2 as [t2_v0 t2]. simpl in KEQ.
+  apply list_app_partition in KEQ;
+    try (intros; eapply tree_n_disjoint_0_pos; eassumption).
+  destruct KEQ as [KEQ1 KEQ2]. f_equal.
+  - destruct t1_v0, t2_v0; trivial2. specialize (VALS 0). simpl in VALS.
+    apply VALS. reflexivity.
+  - eapply tkeys_p_inj.
+    (* VALS *) intros. specialize (VALS (Npos v)). apply VALS. assumption.
+    (* KEQ *) eapply map_inj; trivial2. prove_injective.
+    (* INJ *) prove_injective.
+Qed.
